Package new modifies to avoid explicit use of HS?.h, MR.as_hsref
NOT using taramana_modifies yet, of course.

Epochs.fst lax-typechecks

***NO_CI***

src/tls/TLSMem.fst
@@ -5,15 +5,42 @@ include FStar.HyperStack
 include FStar.ST
 include FStar.All
 
+module MR = FStar.Monotonic.RRef
+module HH = FStar.HyperHeap
+module HS = FStar.HyperStack
+
 let hh_as_ref = HyperHeap.as_ref
+let hh_modifies = HyperHeap.modifies
+let hh_modifies_one = HyperHeap.modifies_one
+
+let hs_modifies_0
+  (r: HH.rid)
+  (h0 h1: HS.mem)
+: Tot Type0
+= HS.modifies_one r h0 h1 /\
+  HH.modifies_rref r !{} (HS.HS?.h h0) (HS.HS?.h h1)
+
+let m_rref_modifies_1
+  (r: MR.rid)
+  (#a:Type)
+  (#b: MR.reln a)
+  (ctr: MR.m_rref r a b)
+  (h0 h1: HS.mem)
+: Tot Type0
+= let ctr_as_href = MR.as_hsref ctr in
+  HS.modifies_one r h0 h1 /\
+  HH.modifies_rref r !{HS.as_ref ctr_as_href} (HS.HS?.h h0) (HS.HS?.h h1)
+
+
 
 (* TODO:
  - regions from Parse
  - colors: replace with stateful operator giving a fresh color
 *)
+(*
+assume val fresh_color: unit -> ST color (requires (fun h -> True)) (ensures (fun h c h1 -> True)) // c `not_in` h /\ c `in` h1)) // TODO: implement
 
-assume val fresh_color: unit -> ST color (requires (fun h -> True)) (ensures (fun h c h1 -> c not in h /\ c in h1)) // TODO: implement
-
+(*
 private
 let tls_color_epoch_color_hs_color =
   let t = fresh_color () in
